CertiGC/verif_create_heap.v
@@ -85,13 +85,13 @@ Proof.
     rewrite sublist_list_repeat by omega. simpl list_repeat at 1.
     rewrite space_array_1_eq. Intros. forward_call (Tsh, h, Z.shiftl 1 16, gv, sh).
     (* make succeed *)
-    + split; [apply writable_share_top|split; [assumption|]].
+    + split; [apply writable_share_top|split; [assumption|]]. rewrite WORD_SIZE_eq.
       split; compute; intros S; inversion S.
     + Intros p0. freeze [0;1;2;4] FR.
       (* change back to "data_at sh heap_type v h" *)
       rewrite <- space_array_1_eq. rewrite sublist_list_repeat by omega.
       change (12 - 1) with 11 at 2. gather_SEP 1 2.
-      remember (p0, (p0, offset_val (4 * Z.shiftl 1 16) p0)) as vh.
+      remember (p0, (p0, offset_val (WORD_SIZE * Z.shiftl 1 16) p0)) as vh.
       remember (vh :: list_repeat (Z.to_nat 11) vn) as vl.
       change (Values.val) with (@val pPGG_VST) in *.
       replace [vh] with (sublist 0 1 vl). 2: {
